FStar.Cardinality.Universes: generalize proof a bit
It works for any larger universe not just +1

ulib/FStar.Cardinality.Universes.fst
@@ -6,11 +6,11 @@ open FStar.Cardinality.Cantor
 (* This type is an injection of all powersets of Type u (i.e. Type u -> bool
 functions) into Type (u+1) *)
 noeq
-type type_powerset : (Type u#a -> bool) -> Type u#(a+1) =
+type type_powerset : (Type u#a -> bool) -> Type u#(max (a+1) b) =
   | Mk : f:(Type u#a -> bool) -> type_powerset f
 
 let aux_inj_type_powerset (f1 f2 : powerset (Type u#a))
-  : Lemma (requires type_powerset f1 == type_powerset f2)
+  : Lemma (requires type_powerset u#a u#b f1 == type_powerset u#a u#b f2)
           (ensures f1 == f2)
 =
   assert (type_powerset f1 == type_powerset f2);
@@ -22,13 +22,14 @@ let aux_inj_type_powerset (f1 f2 : powerset (Type u#a))
 let inj_type_powerset () : Lemma (is_inj type_powerset) =
   Classical.forall_intro_2 (fun f1 -> Classical.move_requires (aux_inj_type_powerset f1))
  
- (* The general structure of this proof is:
-   1- We know there is an injection of powerset(Type(u)) into Type(u+1) (see type_powerset above)
+(* let u' > u be universes. (u' = max(a+1, b), u=a below)
+   The general structure of this proof is:
+   1- We know there is an injection of powerset(Type(u)) into Type(u') (see type_powerset above)
    2- We know there is NO injection from powerset(Type(u)) into Type(u) (see no_inj_powerset)
-   3- Therefore, there cannot be an injection from Type(u+1) into Type(u), otherwise we would
+   3- Therefore, there cannot be an injection from Type(u') into Type(u), otherwise we would
       compose it with the first injection and obtain the second impossible injection.
 *)
-let no_inj_universes (f : Type u#(a+1) -> Type u#a) : Lemma (~(is_inj f)) =
+let no_inj_universes (f : Type u#(max (a+1) b) -> Type u#a) : Lemma (~(is_inj f)) =
   let aux () : Lemma (requires is_inj f) (ensures False) =
     let comp : powerset (Type u#a) -> Type u#a = fun x -> f (type_powerset x) in
     inj_type_powerset ();
@@ -36,3 +37,6 @@ let no_inj_universes (f : Type u#(a+1) -> Type u#a) : Lemma (~(is_inj f)) =
     no_inj_powerset _ comp
   in
   Classical.move_requires aux ()
+
+let no_inj_universes_suc (f : Type u#(a+1) -> Type u#a) : Lemma (~(is_inj f)) =
+  no_inj_universes f
